\section{Homomorphisms and Isomorphisms}

Let $G$ and $H$ be groups.

\Exercise1 Let $\varphi\colon G\to H$ be a homomorphism.
\begin{enumerate}
\item Prove that $\varphi(x^n) = \varphi(x)^n$ for all $n\in\Z^+$.
  \begin{proof}
    We use induction on $n$. The case for $n = 1$ is clear. Suppose
    $\varphi(x^n) = \varphi(x)^n$ for some particular $n\in\Z^+$. Then
    \begin{equation*}
      \varphi(x^{n+1})
      = \varphi(xx^n)
      = \varphi(x)\varphi(x^n)
      = \varphi(x)\varphi(x)^n
      = \varphi(x)^{n+1},
    \end{equation*}
    so the result holds for all $n\in\Z^+$.
  \end{proof}
\item Do part (a) for $n = -1$ and deduce that
  $\varphi(x^n) = \varphi(x)^n$ for all $n\in\Z$.
  \begin{solution}
    Let $1_G$ and $1_H$ denote the identities of $G$ and $H$,
    respectively. Then
    \begin{equation*}
      \varphi(1_G)\varphi(1_G) = \varphi(1_G) = \varphi(1_G)1_H,
    \end{equation*}
    and it follows from the cancellation law that
    $\varphi(1_G) = 1_H$. Since the identity is preserved, we will
    simply use $1$ to denote the identity of both groups from this
    point forward.

    Now, for any $x\in G$,
    \begin{equation*}
      \varphi(x)\varphi(x^{-1}) = \varphi(xx^{-1}) = \varphi(1) = 1,
    \end{equation*}
    which shows that $\varphi(x^{-1}) = \varphi(x)^{-1}$. Then for
    $n\in\Z^+$,
    \begin{equation*}
      \varphi(x^{-n}) = \varphi((x^n)^{-1}) = \varphi(x^n)^{-1}
      = \big(\varphi(x)^n\big)^{-1} = \varphi(x)^{-n}.
    \end{equation*}
    Therefore $\varphi(x^n) = \varphi(x)^n$ holds for all $n\in\Z$.
  \end{solution}
\end{enumerate}
